examples/to_port/queens/queens_WP_NQueensSets_WP_parameter_t3_5.v
@@ -2,28 +2,31 @@
 (* Beware! Only edit allowed sections below    *)
 Require Import BuiltIn.
 Require BuiltIn.
+Require HighOrd.
 Require int.Int.
 Require map.Map.
 
-(* Why3 assumption *)
-Definition unit := unit.
-
-Axiom set : forall (a:Type) {a_WT:WhyType a}, Type.
+Axiom set : forall (a:Type), Type.
 Parameter set_WhyType : forall (a:Type) {a_WT:WhyType a}, WhyType (set a).
 Existing Instance set_WhyType.
 
 Parameter mem: forall {a:Type} {a_WT:WhyType a}, a -> (set a) -> Prop.
 
-(* Why3 assumption *)
-Definition infix_eqeq {a:Type} {a_WT:WhyType a} (s1:(set a)) (s2:(set
-  a)): Prop := forall (x:a), (mem x s1) <-> (mem x s2).
+Parameter infix_eqeq: forall {a:Type} {a_WT:WhyType a}, (set a) -> (set a) ->
+  Prop.
+
+Axiom infix_eqeq_spec : forall {a:Type} {a_WT:WhyType a}, forall (s1:(set a))
+  (s2:(set a)), (infix_eqeq s1 s2) <-> forall (x:a), (mem x s1) <-> (mem x
+  s2).
 
 Axiom extensionality : forall {a:Type} {a_WT:WhyType a}, forall (s1:(set a))
   (s2:(set a)), (infix_eqeq s1 s2) -> (s1 = s2).
 
-(* Why3 assumption *)
-Definition subset {a:Type} {a_WT:WhyType a} (s1:(set a)) (s2:(set
-  a)): Prop := forall (x:a), (mem x s1) -> (mem x s2).
+Parameter subset: forall {a:Type} {a_WT:WhyType a}, (set a) -> (set a) ->
+  Prop.
+
+Axiom subset_spec : forall {a:Type} {a_WT:WhyType a}, forall (s1:(set a))
+  (s2:(set a)), (subset s1 s2) <-> forall (x:a), (mem x s1) -> (mem x s2).
 
 Axiom subset_refl : forall {a:Type} {a_WT:WhyType a}, forall (s:(set a)),
   (subset s s).
@@ -32,27 +35,31 @@ Axiom subset_trans : forall {a:Type} {a_WT:WhyType a}, forall (s1:(set a))
   (s2:(set a)) (s3:(set a)), (subset s1 s2) -> ((subset s2 s3) -> (subset s1
   s3)).
 
+Parameter is_empty: forall {a:Type} {a_WT:WhyType a}, (set a) -> Prop.
+
+Axiom is_empty_spec : forall {a:Type} {a_WT:WhyType a}, forall (s:(set a)),
+  (is_empty s) <-> forall (x:a), ~ (mem x s).
+
 Parameter empty: forall {a:Type} {a_WT:WhyType a}, (set a).
 
-(* Why3 assumption *)
-Definition is_empty {a:Type} {a_WT:WhyType a} (s:(set a)): Prop :=
-  forall (x:a), ~ (mem x s).
-
-Axiom empty_def1 : forall {a:Type} {a_WT:WhyType a}, (is_empty (empty :(set
+Axiom empty_def : forall {a:Type} {a_WT:WhyType a}, (is_empty (empty : (set
   a))).
-
-Axiom mem_empty : forall {a:Type} {a_WT:WhyType a}, forall (x:a), ~ (mem x
-  (empty :(set a))).
 
 Parameter add: forall {a:Type} {a_WT:WhyType a}, a -> (set a) -> (set a).
 
-Axiom add_def1 : forall {a:Type} {a_WT:WhyType a}, forall (x:a) (y:a),
-  forall (s:(set a)), (mem x (add y s)) <-> ((x = y) \/ (mem x s)).
+Axiom add_spec : forall {a:Type} {a_WT:WhyType a}, forall (x:a) (s:(set a)),
+  forall (y:a), (mem y (add x s)) <-> ((y = x) \/ (mem y s)).
 
 Parameter remove: forall {a:Type} {a_WT:WhyType a}, a -> (set a) -> (set a).
 
-Axiom remove_def1 : forall {a:Type} {a_WT:WhyType a}, forall (x:a) (y:a)
-  (s:(set a)), (mem x (remove y s)) <-> ((~ (x = y)) /\ (mem x s)).
+Axiom remove_spec : forall {a:Type} {a_WT:WhyType a}, forall (x:a) (s:(set
+  a)), forall (y:a), (mem y (remove x s)) <-> ((~ (y = x)) /\ (mem y s)).
+
+Axiom add_remove : forall {a:Type} {a_WT:WhyType a}, forall (x:a) (s:(set
+  a)), (mem x s) -> ((add x (remove x s)) = s).
+
+Axiom remove_add : forall {a:Type} {a_WT:WhyType a}, forall (x:a) (s:(set
+  a)), ((remove x (add x s)) = (remove x s)).
 
 Axiom subset_remove : forall {a:Type} {a_WT:WhyType a}, forall (x:a) (s:(set
   a)), (subset (remove x s) s).
@@ -60,27 +67,30 @@ Axiom subset_remove : forall {a:Type} {a_WT:WhyType a}, forall (x:a) (s:(set
 Parameter union: forall {a:Type} {a_WT:WhyType a}, (set a) -> (set a) -> (set
   a).
 
-Axiom union_def1 : forall {a:Type} {a_WT:WhyType a}, forall (s1:(set a))
-  (s2:(set a)) (x:a), (mem x (union s1 s2)) <-> ((mem x s1) \/ (mem x s2)).
+Axiom union_spec : forall {a:Type} {a_WT:WhyType a}, forall (s1:(set a))
+  (s2:(set a)), forall (x:a), (mem x (union s1 s2)) <-> ((mem x s1) \/ (mem x
+  s2)).
 
 Parameter inter: forall {a:Type} {a_WT:WhyType a}, (set a) -> (set a) -> (set
   a).
 
-Axiom inter_def1 : forall {a:Type} {a_WT:WhyType a}, forall (s1:(set a))
-  (s2:(set a)) (x:a), (mem x (inter s1 s2)) <-> ((mem x s1) /\ (mem x s2)).
+Axiom inter_spec : forall {a:Type} {a_WT:WhyType a}, forall (s1:(set a))
+  (s2:(set a)), forall (x:a), (mem x (inter s1 s2)) <-> ((mem x s1) /\ (mem x
+  s2)).
 
 Parameter diff: forall {a:Type} {a_WT:WhyType a}, (set a) -> (set a) -> (set
   a).
 
-Axiom diff_def1 : forall {a:Type} {a_WT:WhyType a}, forall (s1:(set a))
-  (s2:(set a)) (x:a), (mem x (diff s1 s2)) <-> ((mem x s1) /\ ~ (mem x s2)).
+Axiom diff_spec : forall {a:Type} {a_WT:WhyType a}, forall (s1:(set a))
+  (s2:(set a)), forall (x:a), (mem x (diff s1 s2)) <-> ((mem x s1) /\ ~ (mem
+  x s2)).
 
 Axiom subset_diff : forall {a:Type} {a_WT:WhyType a}, forall (s1:(set a))
   (s2:(set a)), (subset (diff s1 s2) s1).
 
 Parameter choose: forall {a:Type} {a_WT:WhyType a}, (set a) -> a.
 
-Axiom choose_def : forall {a:Type} {a_WT:WhyType a}, forall (s:(set a)),
+Axiom choose_spec : forall {a:Type} {a_WT:WhyType a}, forall (s:(set a)),
   (~ (is_empty s)) -> (mem (choose s) s).
 
 Parameter cardinal: forall {a:Type} {a_WT:WhyType a}, (set a) -> Z.
@@ -102,50 +112,48 @@ Axiom cardinal_remove : forall {a:Type} {a_WT:WhyType a}, forall (x:a),
 Axiom cardinal_subset : forall {a:Type} {a_WT:WhyType a}, forall (s1:(set a))
   (s2:(set a)), (subset s1 s2) -> ((cardinal s1) <= (cardinal s2))%Z.
 
+Axiom subset_eq : forall {a:Type} {a_WT:WhyType a}, forall (s1:(set a))
+  (s2:(set a)), (subset s1 s2) -> (((cardinal s1) = (cardinal s2)) ->
+  (infix_eqeq s1 s2)).
+
 Axiom cardinal1 : forall {a:Type} {a_WT:WhyType a}, forall (s:(set a)),
   ((cardinal s) = 1%Z) -> forall (x:a), (mem x s) -> (x = (choose s)).
 
 Parameter min_elt: (set Z) -> Z.
 
-Axiom min_elt_def1 : forall (s:(set Z)), (~ (is_empty s)) -> (mem (min_elt s)
-  s).
-
-Axiom min_elt_def2 : forall (s:(set Z)), (~ (is_empty s)) -> forall (x:Z),
-  (mem x s) -> ((min_elt s) <= x)%Z.
+Axiom min_elt_spec : forall (s:(set Z)), (~ (is_empty s)) -> ((mem
+  (min_elt s) s) /\ forall (x:Z), (mem x s) -> ((min_elt s) <= x)%Z).
 
 Parameter max_elt: (set Z) -> Z.
 
-Axiom max_elt_def1 : forall (s:(set Z)), (~ (is_empty s)) -> (mem (max_elt s)
-  s).
+Axiom max_elt_spec : forall (s:(set Z)), (~ (is_empty s)) -> ((mem
+  (max_elt s) s) /\ forall (x:Z), (mem x s) -> (x <= (max_elt s))%Z).
 
-Axiom max_elt_def2 : forall (s:(set Z)), (~ (is_empty s)) -> forall (x:Z),
-  (mem x s) -> (x <= (max_elt s))%Z.
+Parameter interval: Z -> Z -> (set Z).
 
-Parameter below: Z -> (set Z).
+Axiom interval_spec : forall (l:Z) (r:Z), forall (x:Z), (mem x (interval l
+  r)) <-> ((l <= x)%Z /\ (x < r)%Z).
 
-Axiom below_def : forall (x:Z) (n:Z), (mem x (below n)) <-> ((0%Z <= x)%Z /\
-  (x < n)%Z).
-
-Axiom cardinal_below : forall (n:Z), ((0%Z <= n)%Z ->
-  ((cardinal (below n)) = n)) /\ ((~ (0%Z <= n)%Z) ->
-  ((cardinal (below n)) = 0%Z)).
+Axiom cardinal_interval : forall (l:Z) (r:Z), ((l <= r)%Z ->
+  ((cardinal (interval l r)) = (r - l)%Z)) /\ ((~ (l <= r)%Z) ->
+  ((cardinal (interval l r)) = 0%Z)).
 
 Parameter succ: (set Z) -> (set Z).
 
-Axiom succ_def : forall (s:(set Z)) (i:Z), (mem i (succ s)) <->
+Axiom succ_spec : forall (s:(set Z)), forall (i:Z), (mem i (succ s)) <->
   ((1%Z <= i)%Z /\ (mem (i - 1%Z)%Z s)).
 
 Parameter pred: (set Z) -> (set Z).
 
-Axiom pred_def : forall (s:(set Z)) (i:Z), (mem i (pred s)) <->
+Axiom pred_spec : forall (s:(set Z)), forall (i:Z), (mem i (pred s)) <->
   ((0%Z <= i)%Z /\ (mem (i + 1%Z)%Z s)).
 
 (* Why3 assumption *)
-Inductive ref (a:Type) {a_WT:WhyType a} :=
+Inductive ref (a:Type) :=
   | mk_ref : a -> ref a.
 Axiom ref_WhyType : forall (a:Type) {a_WT:WhyType a}, WhyType (ref a).
 Existing Instance ref_WhyType.
-Implicit Arguments mk_ref [[a] [a_WT]].
+Implicit Arguments mk_ref [[a]].
 
 (* Why3 assumption *)
 Definition contents {a:Type} {a_WT:WhyType a} (v:(ref a)): a :=
@@ -156,81 +164,86 @@ Definition contents {a:Type} {a_WT:WhyType a} (v:(ref a)): a :=
 Parameter n: Z.
 
 (* Why3 assumption *)
-Definition solution := (map.Map.map Z Z).
+Definition solution := (Z -> Z).
 
 (* Why3 assumption *)
-Definition eq_prefix {a:Type} {a_WT:WhyType a} (t:(map.Map.map Z a))
-  (u:(map.Map.map Z a)) (i:Z): Prop := forall (k:Z), ((0%Z <= k)%Z /\
-  (k < i)%Z) -> ((map.Map.get t k) = (map.Map.get u k)).
+Definition eq_prefix {a:Type} {a_WT:WhyType a} (t:(Z -> a)) (u:(Z -> a))
+  (i:Z): Prop := forall (k:Z), ((0%Z <= k)%Z /\ (k < i)%Z) -> ((t k) = (u
+  k)).
 
 (* Why3 assumption *)
-Definition partial_solution (k:Z) (s:(map.Map.map Z Z)): Prop :=
-  forall (i:Z), ((0%Z <= i)%Z /\ (i < k)%Z) -> (((0%Z <= (map.Map.get s
-  i))%Z /\ ((map.Map.get s i) < n)%Z) /\ forall (j:Z), ((0%Z <= j)%Z /\
-  (j < i)%Z) -> ((~ ((map.Map.get s i) = (map.Map.get s j))) /\
-  ((~ (((map.Map.get s i) - (map.Map.get s j))%Z = (i - j)%Z)) /\
-  ~ (((map.Map.get s i) - (map.Map.get s j))%Z = (j - i)%Z)))).
+Definition partial_solution (k:Z) (s:(Z -> Z)): Prop := forall (i:Z),
+  ((0%Z <= i)%Z /\ (i < k)%Z) -> (((0%Z <= (s i))%Z /\ ((s i) < n)%Z) /\
+  forall (j:Z), ((0%Z <= j)%Z /\ (j < i)%Z) -> ((~ ((s i) = (s j))) /\
+  ((~ (((s i) - (s j))%Z = (i - j)%Z)) /\ ~ (((s i) - (s
+  j))%Z = (j - i)%Z)))).
 
-Axiom partial_solution_eq_prefix : forall (u:(map.Map.map Z Z))
-  (t:(map.Map.map Z Z)) (k:Z), (partial_solution k t) -> ((eq_prefix t u
-  k) -> (partial_solution k u)).
+Axiom partial_solution_eq_prefix : forall (u:(Z -> Z)) (t:(Z -> Z)) (k:Z),
+  (partial_solution k t) -> ((eq_prefix t u k) -> (partial_solution k u)).
 
 (* Why3 assumption *)
-Definition lt_sol (s1:(map.Map.map Z Z)) (s2:(map.Map.map Z Z)): Prop :=
-  exists i:Z, ((0%Z <= i)%Z /\ (i < n)%Z) /\ ((eq_prefix s1 s2 i) /\
-  ((map.Map.get s1 i) < (map.Map.get s2 i))%Z).
+Definition lt_sol (s1:(Z -> Z)) (s2:(Z -> Z)): Prop := exists i:Z,
+  ((0%Z <= i)%Z /\ (i < n)%Z) /\ ((eq_prefix s1 s2 i) /\ ((s1 i) < (s2
+  i))%Z).
 
 (* Why3 assumption *)
-Definition solutions := (map.Map.map Z (map.Map.map Z Z)).
+Definition solutions := (Z -> (Z -> Z)).
 
 (* Why3 assumption *)
-Definition sorted (s:(map.Map.map Z (map.Map.map Z Z))) (a:Z) (b:Z): Prop :=
-  forall (i:Z) (j:Z), (((a <= i)%Z /\ (i < j)%Z) /\ (j < b)%Z) -> (lt_sol
-  (map.Map.get s i) (map.Map.get s j)).
+Definition sorted (s:(Z -> (Z -> Z))) (a:Z) (b:Z): Prop := forall (i:Z)
+  (j:Z), ((a <= i)%Z /\ ((i < j)%Z /\ (j < b)%Z)) -> (lt_sol (s i) (s j)).
 
-Axiom no_duplicate : forall (s:(map.Map.map Z (map.Map.map Z Z))) (a:Z)
-  (b:Z), (sorted s a b) -> forall (i:Z) (j:Z), (((a <= i)%Z /\ (i < j)%Z) /\
-  (j < b)%Z) -> ~ (eq_prefix (map.Map.get s i) (map.Map.get s j) n).
+Axiom no_duplicate : forall (s:(Z -> (Z -> Z))) (a:Z) (b:Z), (sorted s a
+  b) -> forall (i:Z) (j:Z), ((a <= i)%Z /\ ((i < j)%Z /\ (j < b)%Z)) ->
+  ~ (eq_prefix (s i) (s j) n).
 
 (* Why3 goal *)
-Theorem WP_parameter_t3 : forall (a:(set Z)) (b:(set Z)) (c:(set Z)),
-  forall (s:Z) (sol:(map.Map.map Z (map.Map.map Z Z))) (k:Z)
-  (col:(map.Map.map Z Z)), ((0%Z <= k)%Z /\ (((k + (cardinal a))%Z = n) /\
-  ((0%Z <= s)%Z /\ ((forall (i:Z), (mem i a) <-> (((0%Z <= i)%Z /\
-  (i < n)%Z) /\ forall (j:Z), ((0%Z <= j)%Z /\ (j < k)%Z) ->
-  ~ ((map.Map.get col j) = i))) /\ ((forall (i:Z), (0%Z <= i)%Z -> ((~ (mem i
-  b)) <-> forall (j:Z), ((0%Z <= j)%Z /\ (j < k)%Z) -> ~ ((map.Map.get col
+Theorem VC_t3 : forall (col:(Z -> Z)) (k:Z) (sol:(Z -> (Z -> Z))) (s:Z),
+  forall (a:(set Z)) (b:(set Z)) (c:(set Z)), ((0%Z <= k)%Z /\
+  (((k + (cardinal a))%Z = n) /\ ((0%Z <= s)%Z /\ ((forall (i:Z), (mem i
+  a) <-> (((0%Z <= i)%Z /\ (i < n)%Z) /\ forall (j:Z), ((0%Z <= j)%Z /\
+  (j < k)%Z) -> ~ ((col j) = i))) /\ ((forall (i:Z), (0%Z <= i)%Z -> ((~ (mem
+  i b)) <-> forall (j:Z), ((0%Z <= j)%Z /\ (j < k)%Z) -> ~ ((col
   j) = ((i + j)%Z - k)%Z))) /\ ((forall (i:Z), (0%Z <= i)%Z -> ((~ (mem i
-  c)) <-> forall (j:Z), ((0%Z <= j)%Z /\ (j < k)%Z) -> ~ ((map.Map.get col
-  j) = ((i + k)%Z - j)%Z))) /\ (partial_solution k col))))))) ->
-  ((~ (is_empty a)) -> forall (f:Z) (e:(set Z)) (s1:Z) (sol1:(map.Map.map Z
-  (map.Map.map Z Z))) (k1:Z) (col1:(map.Map.map Z Z)), (((f = (s1 - s)%Z) /\
-  (0%Z <= (s1 - s)%Z)%Z) /\ ((k1 = k) /\ ((subset e (diff (diff a b) c)) /\
-  ((partial_solution k1 col1) /\ ((sorted sol1 s s1) /\ ((forall (i:Z) (j:Z),
-  (mem i (diff (diff (diff a b) c) e)) -> ((mem j e) -> (i < j)%Z)) /\
-  ((forall (t:(map.Map.map Z Z)), ((partial_solution n t) /\ ((eq_prefix col1
-  t k1) /\ (mem (map.Map.get t k1) (diff (diff (diff a b) c) e)))) <->
-  exists i:Z, ((s <= i)%Z /\ (i < s1)%Z) /\ (eq_prefix t (map.Map.get sol1 i)
+  c)) <-> forall (j:Z), ((0%Z <= j)%Z /\ (j < k)%Z) -> ~ ((col
+  j) = ((i + k)%Z - j)%Z))) /\ (partial_solution k col))))))) -> (((is_empty
+  a) <-> forall (x:Z), ~ (mem x a)) -> ((~ (is_empty a)) -> let o := (diff a
+  b) in ((forall (x:Z), (mem x o) <-> ((mem x a) /\ ~ (mem x b))) ->
+  let o1 := (diff o c) in ((forall (x:Z), (mem x o1) <-> ((mem x o) /\ ~ (mem
+  x c))) -> forall (f:Z) (e:(set Z)) (s1:Z) (sol1:(Z -> (Z -> Z))) (k1:Z)
+  (col1:(Z -> Z)), (((f = (s1 - s)%Z) /\ (0%Z <= (s1 - s)%Z)%Z) /\
+  ((k1 = k) /\ ((subset e (diff (diff a b) c)) /\ ((partial_solution k1
+  col1) /\ ((sorted sol1 s s1) /\ ((forall (i:Z) (j:Z), (mem i (diff o1
+  e)) -> ((mem j e) -> (i < j)%Z)) /\ ((forall (t:(Z -> Z)),
+  ((partial_solution n t) /\ ((eq_prefix col1 t k1) /\ (mem (t k1) (diff o1
+  e)))) <-> exists i:Z, ((s <= i)%Z /\ (i < s1)%Z) /\ (eq_prefix t (sol1 i)
   n)) /\ ((eq_prefix col col1 k1) /\ (eq_prefix sol sol1 s))))))))) ->
-  ((~ (is_empty e)) -> let d := (min_elt e) in forall (col2:(map.Map.map Z
-  Z)), (col2 = (map.Map.set col1 k1 d)) -> forall (k2:Z),
-  (k2 = (k1 + 1%Z)%Z) -> let o := (remove d a) in (((0%Z <= k2)%Z /\
-  (((k2 + (cardinal o))%Z = n) /\ ((0%Z <= s1)%Z /\ ((forall (i:Z), (mem i
-  o) <-> (((0%Z <= i)%Z /\ (i < n)%Z) /\ forall (j:Z), ((0%Z <= j)%Z /\
-  (j < k2)%Z) -> ~ ((map.Map.get col2 j) = i))) /\ ((forall (i:Z),
-  (0%Z <= i)%Z -> ((~ (mem i (succ (add d b)))) <-> forall (j:Z),
-  ((0%Z <= j)%Z /\ (j < k2)%Z) -> ~ ((map.Map.get col2
-  j) = ((i + j)%Z - k2)%Z))) /\ ((forall (i:Z), (0%Z <= i)%Z -> ((~ (mem i
-  (pred (add d c)))) <-> forall (j:Z), ((0%Z <= j)%Z /\ (j < k2)%Z) ->
-  ~ ((map.Map.get col2 j) = ((i + k2)%Z - j)%Z))) /\ (partial_solution k2
-  col2))))))) -> forall (s2:Z) (sol2:(map.Map.map Z (map.Map.map Z Z)))
-  (k3:Z) (col3:(map.Map.map Z Z)), ((0%Z <= (s2 - s1)%Z)%Z /\ ((k3 = k2) /\
-  ((sorted sol2 s1 s2) /\ ((forall (t:(map.Map.map Z Z)), ((partial_solution
-  n t) /\ (eq_prefix col3 t k3)) <-> exists i:Z, ((s1 <= i)%Z /\
-  (i < s2)%Z) /\ (eq_prefix t (map.Map.get sol2 i) n)) /\ ((eq_prefix col2
-  col3 k3) /\ (eq_prefix sol1 sol2 s1)))))) -> forall (f1:Z),
-  (f1 = (f + (s2 - s1)%Z)%Z) -> forall (k4:Z), (k4 = (k3 - 1%Z)%Z) ->
-  forall (e1:(set Z)), (e1 = (remove d e)) -> (sorted sol2 s s2)))).
+  (((is_empty e) <-> forall (x:Z), ~ (mem x e)) -> ((~ (is_empty e)) ->
+  let d := (min_elt e) in (((mem d e) /\ forall (x:Z), (mem x e) ->
+  (d <= x)%Z) -> forall (col2:(Z -> Z)), (col2 = (map.Map.set col1 k1 d)) ->
+  forall (k2:Z), (k2 = (k1 + 1%Z)%Z) -> let o2 := (add d c) in
+  ((forall (y:Z), (mem y o2) <-> ((y = d) \/ (mem y c))) -> ((forall (i:Z),
+  (mem i (pred o2)) <-> ((0%Z <= i)%Z /\ (mem (i + 1%Z)%Z o2))) -> let o3 :=
+  (add d b) in ((forall (y:Z), (mem y o3) <-> ((y = d) \/ (mem y b))) ->
+  ((forall (i:Z), (mem i (succ o3)) <-> ((1%Z <= i)%Z /\ (mem (i - 1%Z)%Z
+  o3))) -> ((forall (y:Z), (mem y (remove d a)) <-> ((~ (y = d)) /\ (mem y
+  a))) -> forall (s2:Z) (sol2:(Z -> (Z -> Z))) (k3:Z) (col3:(Z -> Z)),
+  ((0%Z <= (s2 - s1)%Z)%Z /\ ((k3 = k2) /\ ((sorted sol2 s1 s2) /\
+  ((forall (t:(Z -> Z)), ((partial_solution n t) /\ (eq_prefix col3 t
+  k3)) <-> exists i:Z, ((s1 <= i)%Z /\ (i < s2)%Z) /\ (eq_prefix t (sol2 i)
+  n)) /\ ((eq_prefix col2 col3 k3) /\ (eq_prefix sol1 sol2 s1)))))) ->
+  forall (f1:Z), (f1 = (f + (s2 - s1)%Z)%Z) -> forall (k4:Z),
+  (k4 = (k3 - 1%Z)%Z) -> let o4 := (remove d e) in ((forall (y:Z), (mem y
+  o4) <-> ((~ (y = d)) /\ (mem y e))) -> forall (e1:(set Z)), (e1 = o4) ->
+  (sorted sol2 s s2)))))))))))))).
+intros col k sol s a b c (h1,(h2,(h3,(h4,(h5,(h6,h7)))))) h8 h9 o h10 o1 h11
+f e s1 sol1 k1 col1 ((h12,h13),(h14,(h15,(h16,(h17,(h18,(h19,(h20,h21))))))))
+h22 h23 d (h24,h25) col2 h26 k2 h27 o2 h28 h29 o3 h30 h31 h32 s2 sol2 k3 col3
+(h33,(h34,(h35,(h36,(h37,h38))))) f1 h39 k4 h40 o4 h41 e1 h42.
+
+Qed.
+
+(* Unused content named WP_parameter_t3
 intros a b c s sol k col (h1,(h2,(h3,(h4,(h5,(h6,h7)))))) h8 f e s1
         sol1 k1 col1 ((h9,h10),(h11,(h12,(h13,(h14,(h15,(h16,(h17,h18))))))))
         h19 d col2 h20 k2 h21 o (h22,(h23,(h24,(h25,(h26,(h27,h28)))))) s2
@@ -281,5 +294,4 @@ rewrite <- h33; try omega.
 subst col2; rewrite Map.Select_eq; try omega.
 generalize (min_elt_def1 e); intuition.
 Qed.
-
-
+ *)
